aes/equiv_encryption.v
@@ -2,58 +2,11 @@ Require Import aes.spec_encryption_LL.
 Require Import aes.spec_AES256_HL.
 Require Import aes.tablesLL.
 Require Import aes.GF_ops_LL.
+Require Import aes.conv_HL_to_LL.
+Require Import aes.bitfiddling.
+Require Import aes.list_lemmas.
+Require Import aes.equiv_GF_ops.
 Require Import List. Import ListNotations.
-
-(* Note: In the standard, the 4x4 matrix is filled with bytes column-wise, but the
-   high-level spec fills it row-wise, so we have to transpose in the right spots *)
-
-Definition state_to_list (s : state) : list int :=
-  match transpose s with
-  | ((b11, b12, b13, b14), (b21, b22, b23, b24), (b31, b32, b33, b34), (b41, b42, b43, b44)) =>
-    [ b11; b12; b13; b14 ;  b21; b22; b23; b24 ;  b31; b32; b33; b34 ;  b41; b42; b43; b44 ]
-  end.
-
-Definition list_to_state (l : list int) : state := transpose
-  match l with
-  | [ b11; b12; b13; b14 ;  b21; b22; b23; b24 ;  b31; b32; b33; b34 ;  b41; b42; b43; b44 ] =>
-    ((b11, b12, b13, b14), (b21, b22, b23, b24), (b31, b32, b33, b34), (b41, b42, b43, b44))
-  (* should not happen: *)
-  | _ => let z4 := (Int.zero, Int.zero, Int.zero, Int.zero) in
-         (z4, z4, z4, z4)
-  end.
-
-Definition word_to_int (w : word) : int :=
-  match w with (b0, b1, b2, b3) =>
-    (Int.or (Int.or (Int.or
-             b0
-    (Int.shl b1 (Int.repr  8)))
-    (Int.shl b2 (Int.repr 16)))
-    (Int.shl b3 (Int.repr 24)))
-  end.
-
-(*
-Definition int_to_word (x : int) : word := (
-  (Int.and           x                (Int.repr 255)),
-  (Int.and (Int.shru x (Int.repr  8)) (Int.repr 255)),
-  (Int.and (Int.shru x (Int.repr 16)) (Int.repr 255)),
-  (Int.and (Int.shru x (Int.repr 24)) (Int.repr 255))
-).
-
-Definition four_ints_to_state (s : four_ints) : state := transpose match s with
-| (c0, (c1, (c2, c3))) => (int_to_word c0, int_to_word c1, int_to_word c2, int_to_word c3)
-end.
-*)
-
-Definition state_to_four_ints (s : state) : four_ints := match transpose s with
-| (c0, c1, c2, c3) => (word_to_int c0, (word_to_int c1, (word_to_int c2, word_to_int c3)))
-end.
-
-Definition block_to_ints (b : block) : list int :=
-  match b with (w0, w1, w2, w3) => [word_to_int w0; word_to_int w1; word_to_int w2; word_to_int w3] end.
-
-Definition blocks_to_ints (blocks : list block) : list int := flat_map block_to_ints blocks.
-
-Definition blocks_to_Zwords (blocks : list block) : list Z := map Int.unsigned (blocks_to_ints blocks).
 
 Lemma split_quad_eq: forall {T : Type} (c0 c1 c2 c3 c0' c1' c2' c3' : T),
   c0 = c0' -> c1 = c1' -> c2 = c2' -> c3 = c3' -> (c0, c1, c2, c3) = (c0', c1', c2', c3').
@@ -67,52 +20,6 @@ Lemma split_4eq: forall (T : Type) (c0 c1 c2 c3 c0' c1' c2' c3' : T),
 Proof.
   intros. inversion H. subst. auto.
 Qed.
-
-Lemma byte0_word_to_int: forall b0 b1 b2 b3,
-  byte0 (word_to_int (b0, b1, b2, b3)) = Int.unsigned b0.
-Admitted.
-
-Lemma byte1_word_to_int: forall b0 b1 b2 b3,
-  byte1 (word_to_int (b0, b1, b2, b3)) = Int.unsigned b1.
-Admitted.
-
-Lemma byte2_word_to_int: forall b0 b1 b2 b3,
-  byte2 (word_to_int (b0, b1, b2, b3)) = Int.unsigned b2.
-Admitted.
-
-Lemma byte3_word_to_int: forall b0 b1 b2 b3,
-  byte3 (word_to_int (b0, b1, b2, b3)) = Int.unsigned b3.
-Admitted.
-
-Ltac eval_list l :=
-  let l' := eval hnf in l in lazymatch l' with
-  | ?h :: ?tl => let tl' := eval_list tl in constr:(h :: tl')
-  | (@nil ?T) => constr:(@nil T)
-  end.
-
-Lemma xor_byte0_with_FSb: forall b0 b1 b2 b3 i,
-  Int.xor (word_to_int (b0, b1, b2, b3)) (Znth i tablesLL.FSb Int.zero)
-  = word_to_int ((Int.xor b0 (Znth i tablesLL.FSb Int.zero)), b1, b2, b3).
-Admitted.
-
-Lemma xor_byte1_with_FSb: forall b0 b1 b2 b3 i,
-  Int.xor (word_to_int (b0, b1, b2, b3)) (Int.shl (Znth i tablesLL.FSb Int.zero) (Int.repr 8))
-  = word_to_int (b0, (Int.xor b1 (Znth i tablesLL.FSb Int.zero)), b2, b3).
-Admitted.
-
-Lemma xor_byte2_with_FSb: forall b0 b1 b2 b3 i,
-  Int.xor (word_to_int (b0, b1, b2, b3)) (Int.shl (Znth i tablesLL.FSb Int.zero) (Int.repr 16))
-  = word_to_int (b0, b1, (Int.xor b2 (Znth i tablesLL.FSb Int.zero)), b3).
-Admitted.
-
-Lemma xor_byte3_with_FSb: forall b0 b1 b2 b3 i,
-  Int.xor (word_to_int (b0, b1, b2, b3)) (Int.shl (Znth i tablesLL.FSb Int.zero) (Int.repr 24))
-  = word_to_int (b0, b1, b2, (Int.xor b3 (Znth i tablesLL.FSb Int.zero))).
-Admitted.
-
-Lemma equiv_sbox: forall b,
-  Znth (Int.unsigned b) tablesLL.FSb Int.zero = look_sbox b.
-Admitted.
 
 Lemma get_uint32_le_sublist: forall i l,
   0 <= i <= Zlength l - 4 ->
@@ -135,13 +42,6 @@ Proof.
   do 4 rewrite Int.repr_unsigned.
   reflexivity.
 Qed.
-
-Lemma xor_word_to_int: forall a0 a1 a2 a3 b0 b1 b2 b3,
-  Int.xor (word_to_int (a0, a1, a2, a3)) (word_to_int (b0, b1, b2, b3))
-  = word_to_int ((Int.xor a0 b0), (Int.xor a1 b1), (Int.xor a2 b2), (Int.xor a3 b3)).
-Proof.
-  intros. unfold word_to_int.
-Admitted.
 
 Lemma initial_round_equiv: forall S K,
   (mbed_tls_initial_add_round_key
@@ -205,15 +105,6 @@ Proof.
   reflexivity.
 Qed.
 
-Lemma Znth_fill_list: forall {T: Type} (i n: Z) (f: Z -> T) (d: T),
-  0 <= i < n ->
-  Znth i (fill_list n f) d = f i.
-Admitted.
-
-Lemma rot8_word_to_int: forall b0 b1 b2 b3,
-  rot8 (word_to_int (b0, b1, b2, b3)) = word_to_int (b3, b0, b1, b2).
-Admitted.
-
 Definition FT0b0(i: Z): int := GF_ops_LL.times2 (Znth i FSb Int.zero).
 Definition FT0b1(i: Z): int := Znth i FSb Int.zero.
 Definition FT0b2(i: Z): int := Znth i FSb Int.zero.
@@ -221,15 +112,6 @@ Definition FT0b3(i: Z): int := GF_ops_LL.times3 (Znth i FSb Int.zero).
 (* Note: according to calc_FT0, it should FT0b3 is
      (Int.and (Int.xor (GF_ops_LL.times2 (Znth i FSb Int.zero)) (Znth i FSb Int.zero)) (Int.repr 255))
    but we prefer to use an equivalent "medium-level" formulation *)
-
-Lemma mask_byte_nop: forall i,
-  0 <= Int.unsigned i < 256 ->
-  Int.and i (Int.repr 255) = i.
-Admitted.
-
-Lemma FSb_range: forall i,
-  0 <= Int.unsigned (Znth i FSb Int.zero) < 256.
-Admitted.
 
 Lemma times3_times2: forall i,
   0 <= Int.unsigned i < 256 ->
@@ -253,11 +135,9 @@ Proof.
   Transparent calc_FT0. unfold calc_FT0.
   unfold word_to_int.
   unfold FT0b0, FT0b1, FT0b2, FT0b3.
-  rewrite Int.xor_is_or by admit.
-  rewrite Int.xor_is_or by admit.
-  rewrite Int.xor_is_or by admit.
+  rewrite xor_is_or_4_bytes.
   f_equal. f_equal. apply times3_times2. apply FSb_range.
-Admitted.
+Qed.
 
 Lemma calc_FT1_expose_bytes: forall i,
   0 <= i < 256 ->
@@ -291,16 +171,6 @@ Proof.
   do 3 rewrite rot8_word_to_int.
   reflexivity.
 Qed.
-
-Lemma times2_equiv: forall b,
-  0 <= Int.unsigned b < 256 ->
-  times2 b = ff_mult (Int.repr 2) b.
-Admitted.
-
-Lemma times3_equiv: forall b,
-  0 <= Int.unsigned b < 256 ->
-  times3 b = ff_mult (Int.repr 3) b.
-Admitted.
 
 Lemma split_quad_eq': forall {T : Type} (c0 c1 c2 c3 c0' c1' c2' c3' : T),
   c0 = c0' -> c1 = c1' -> c2 = c2' -> c3 = c3' -> (c0, (c1, (c2, c3))) = (c0', (c1', (c2', c3'))).
